\documentclass{article}
\usepackage[utf8]{inputenc}
\usepackage[english]{babel}
\usepackage[]{amsthm}
\usepackage[]{amssymb}
\usepackage[]{amsmath}

\title{ISyE/Math/CS/Stat 525 â€“ Linear Optimization\\Spring 2021\\Homework 1}
\author{ZIJIE ZHANG, JIACHENG DENG}
\date\today

\begin{document}
\maketitle

\section*{Exercise 1}
	\begin{proof}
		For every $x, y\in \mathbb{R}^n$ and every $\lambda \in [0,1]$
		\begin{align*}
			f(\lambda x + (1-\lambda) y)
			&=\sum_{i=1}^m f_i(\lambda x + (1-\lambda) y)\\
			&\leqslant \sum_{i=1}^m \lambda f_i(x) + (1-\lambda) f_i(y)\\
			&=\lambda \sum_{i=1}^m f_i(x) + (1-\lambda)\sum_{i=1}^m f_i(y)\\
			&=\lambda f(x) + (1-\lambda)f(y)
		\end{align*}
		$f$ is convex.
	\end{proof}
\section*{Exercise 8}
	\begin{proof}
		\begin{itemize}
			\item[(a)]
			\begin{align*}
				\min\quad & c'(x^+ - x^-)+d'y\\
				\mbox{s.t.}\quad
				& A(x^+ - x^-)+By+z-b=0\\
				& x^+ + x^- - y=0\\
				& x^+, x^-, z\geqslant 0
			\end{align*}
			\item[(b)]
				For every feasible solution to the original problem,
				$$(x, y) = (x^+-x^-, y)$$
				There exists a feasible solution to reformulation problem.
		\end{itemize}
	\end{proof}
\section*{Exercise 9}
	\begin{proof}
		\begin{align*}
			\min\quad & \left\Vert I-I^* \right\Vert_2\\
			\mbox{s.t.}\quad
			& I = A * P\\
			\mbox{where}\quad
			& A_{ij} = a_{ij}, P_j = p_j
		\end{align*}
	\end{proof}
\section*{Exercise 11}
	\begin{proof}

	\end{proof}
\section*{Exercise 12}
	\begin{proof}

	\end{proof}

\end{document}